src/Examples/CacheADT/CacheSpec.v
@@ -1,6 +1,6 @@
 Require Import Coq.Strings.String Coq.omega.Omega Coq.Lists.List Coq.Logic.FunctionalExtensionality Coq.Sets.Ensembles
         Fiat.Computation Fiat.ADT Fiat.ADTRefinement Fiat.ADTNotation Fiat.ADTRefinement.BuildADTRefinements
-        ADTExamples.CacheADT.KVEnsembles.
+        Examples.CacheADT.KVEnsembles.
 
 Open Scope string.
 
