src/Examples/ExtractingFiniteSetsExamples.v
@@ -1,5 +1,5 @@
 Require Import Fiat.FiniteSetADTs.FiniteSetADTImplementation.
-Require Import ADTExamples.FiniteSetsExamples.
+Require Import Examples.FiniteSetsExamples.
 
 Require Import Bedrock.Platform.Facade.DFacadeToBedrock.
 Require Import Bedrock.Platform.Facade.examples.FiatADTs.
