src/Examples/SumUniqueAMD64.v
@@ -1,4 +1,4 @@
-Require Import Bedrock AMD64_gas ADTExamples.ExtractingFiniteSetsExamples.
+Require Import Bedrock AMD64_gas Examples.ExtractingFiniteSetsExamples.
 
 Definition compiled := moduleS sumUnique.all.
 Recursive Extraction compiled.
